vale/code/arch/x64/interop/Vale.Wrapper.X64.Cpuid.fst
@@ -29,3 +29,6 @@ let check_sse () =
   let x, _ = Vale.Stdcalls.X64.Cpuid.check_sse () in //This is a call to the interop wrapper
   x
 
+let check_rdrand () =
+  let x, _ = Vale.Stdcalls.X64.Cpuid.check_rdrand () in //This is a call to the interop wrapper
+  x
