providers/evercrypt/fst/EverCrypt.AutoConfig2.fst
@@ -43,6 +43,8 @@ let cpu_has_sse: cached_flag Vale.X64.CPU_Features_s.sse_enabled =
   B.gcmalloc_of_list HS.root [ false ]
 let cpu_has_movbe: cached_flag Vale.X64.CPU_Features_s.movbe_enabled =
   B.gcmalloc_of_list HS.root [ false ]
+let cpu_has_rdrand: cached_flag Vale.X64.CPU_Features_s.rdrand_enabled =
+  B.gcmalloc_of_list HS.root [ false ]
 
 let user_wants_hacl: eternal_pointer bool = B.gcmalloc_of_list HS.root [ SC.hacl ]
 let user_wants_vale: eternal_pointer bool = B.gcmalloc_of_list HS.root [ SC.vale ]
@@ -63,6 +65,7 @@ let has_bmi2 = mk_getter cpu_has_bmi2
 let has_adx = mk_getter cpu_has_adx
 let has_sse = mk_getter cpu_has_sse
 let has_movbe = mk_getter cpu_has_movbe
+let has_rdrand = mk_getter cpu_has_rdrand
 
 let wants_vale () = B.recall user_wants_vale; B.index user_wants_vale 0ul
 let wants_hacl () = B.recall user_wants_hacl; B.index user_wants_hacl 0ul
@@ -78,7 +81,8 @@ let fp_cpu_flags () =
   B.loc_buffer cpu_has_bmi2 `B.loc_union`
   B.loc_buffer cpu_has_adx `B.loc_union`
   B.loc_buffer cpu_has_sse `B.loc_union`
-  B.loc_buffer cpu_has_movbe
+  B.loc_buffer cpu_has_movbe `B.loc_union`
+  B.loc_buffer cpu_has_rdrand
 
 let fp () =
   fp_cpu_flags() `B.loc_union`
@@ -97,12 +101,13 @@ let recall () =
   B.recall cpu_has_adx;
   B.recall cpu_has_sse;
   B.recall cpu_has_movbe;
+  B.recall cpu_has_rdrand;
   B.recall user_wants_hacl;
   B.recall user_wants_vale;
   B.recall user_wants_openssl;
   B.recall user_wants_bcrypt
 
-#set-options "--z3rlimit 400"
+#set-options "--z3rlimit 500"
 let init () =
   // TODO: use an && here once macros are improved
   let h0 = ST.get () in
@@ -139,6 +144,10 @@ let init () =
       if Vale.Wrapper.X64.Cpuid.check_movbe () <> 0UL then begin
         B.recall cpu_has_movbe;
         B.upd cpu_has_movbe 0ul true
+      end;
+      if Vale.Wrapper.X64.Cpuid.check_rdrand () <> 0UL then begin
+        B.recall cpu_has_rdrand;
+        B.upd cpu_has_rdrand 0ul true
       end
     end;
   let h1 = ST.get () in
@@ -171,6 +180,7 @@ let disable_aesni () = B.recall cpu_has_aesni; B.upd cpu_has_aesni 0ul false
 let disable_pclmulqdq () = B.recall cpu_has_pclmulqdq; B.upd cpu_has_pclmulqdq 0ul false
 let disable_sse () = B.recall cpu_has_sse; B.upd cpu_has_sse 0ul false
 let disable_movbe () = B.recall cpu_has_movbe; B.upd cpu_has_movbe 0ul false
+let disable_rdrand () = B.recall cpu_has_rdrand; B.upd cpu_has_rdrand 0ul false
 let disable_vale = mk_disabler user_wants_vale
 let disable_hacl = mk_disabler user_wants_hacl
 let disable_openssl = mk_disabler user_wants_openssl
