vale/specs/hardware/Vale.X64.CPU_Features_s.fst
@@ -15,6 +15,7 @@ assume val sse2_enabled : bool       // CPUID.01H:EDX.SSE2[bit 26]
 assume val ssse3_enabled : bool      // CPUID.01H:ECX.SSSE3[bit 9]
 assume val sse4_1_enabled : bool     // CPUID.01H:ECX.SSE4.1[bit 19]
 assume val movbe_enabled : bool      // CPUID.01H.ECX.MOVBE[bit 22]
+assume val rdrand_enabled : bool     // CPUID.01H.ECX.RDRAND[bit 30] = 0
 
 let sse_enabled : bool = sse2_enabled && ssse3_enabled && sse4_1_enabled
 
@@ -28,6 +29,7 @@ assume val cpuid_features (u:unit) :
          (forall rcx . {:pattern (cpuid rRcx 1 rcx)} (Vale.Def.Types_s.iand (cpuid rRcx 1 rcx) (pow2_norm 9)  > 0) = ssse3_enabled) /\
          (forall rcx . {:pattern (cpuid rRcx 1 rcx)} (Vale.Def.Types_s.iand (cpuid rRcx 1 rcx) (pow2_norm 19)  > 0) = sse4_1_enabled) /\
          (forall rcx . {:pattern (cpuid rRcx 1 rcx)} (Vale.Def.Types_s.iand (cpuid rRcx 1 rcx) (pow2_norm 22)  > 0) = movbe_enabled) /\
+         (forall rcx . {:pattern (cpuid rRcx 1 rcx)} (Vale.Def.Types_s.iand (cpuid rRcx 1 rcx) (pow2_norm 30)  > 0) = rdrand_enabled) /\
          (Vale.Def.Types_s.iand (cpuid rRbx 7 0) (pow2_norm  5) > 0) = avx2_enabled /\
          (Vale.Def.Types_s.iand (cpuid rRbx 7 0) (pow2_norm  8) > 0) = bmi2_enabled /\
          (Vale.Def.Types_s.iand (cpuid rRbx 7 0) (pow2_norm 19) > 0) = adx_enabled /\
